Partial update to Interop to support arbitrary buffers

vale/code/arch/x64/Interop.fst
@@ -15,9 +15,14 @@ open X64.Bytes_Semantics
 
 (* Write a buffer in the vale memory *)
 
-let rec write_vale_mem (contents:Seq.seq UInt8.t) (length:nat{length = FStar.Seq.Base.length contents}) addr (i:nat{i <= length}) 
-      (curr_heap:heap{forall j. {:pattern (Seq.index contents j)} 
-	0 <= j /\ j < i ==> curr_heap.[addr+j] == UInt8.v (Seq.index contents j)}) : Tot heap (decreases %[sub length i]) =
+let rec write_vale_mem 
+  (contents:Seq.seq UInt8.t)
+  (length:nat{length = FStar.Seq.Base.length contents}) 
+  addr 
+  (i:nat{i <= length}) 
+  (curr_heap:heap{forall j. {:pattern (Seq.index contents j)} 
+	0 <= j /\ j < i ==> curr_heap.[addr+j] == UInt8.v (Seq.index contents j)}) 
+  : Tot heap (decreases %[sub length i]) =
     if i >= length then curr_heap
     else (
       let heap = curr_heap.[addr + i] <- UInt8.v (FStar.Seq.index contents i) in
@@ -108,57 +113,57 @@ let rec monotone_domain_write_vale_mem
 #set-options "--z3rlimit 40"
 
 let correct_down_p_cancel mem (addrs:addr_map) heap (p:b8) : Lemma
-  (forall p'. p == p' ==>       
-      (let length = B.length p in
-      let contents = B.as_seq mem p in
+  (forall p'. p === p' ==>       
+      (let length = B.length p.b in
+      let contents = B.as_seq mem p.b in
       let addr = addrs p in
       let new_heap = write_vale_mem contents length addr 0 heap in
       correct_down_p mem addrs new_heap p')) = 
   let rec aux (p':b8) : Lemma 
-    (p == p'  ==> (let length = B.length p in
-      let contents = B.as_seq mem p in
+    (requires p === p')
+    (ensures (let length = B.length p.b in
+      let contents = B.as_seq mem p.b in
       let addr = addrs p in
       let new_heap = write_vale_mem contents length addr 0 heap in
       correct_down_p mem addrs new_heap p')) =
-        let length = B.length p in
-        let contents = B.as_seq mem p in
+        let length = B.length p.b in
+        let contents = B.as_seq mem p.b in
         let addr = addrs p in
         let new_heap = write_vale_mem contents length addr 0 heap in
 	load_store_write_vale_mem contents length addr 0 heap
   in
-  Classical.forall_intro aux
+  Classical.forall_intro (Classical.move_requires aux)
       
+
 let correct_down_p_frame mem (addrs:addr_map) (heap:heap) (p:b8) : Lemma
-  (forall p'. disjoint p p' /\ correct_down_p mem addrs heap p' ==>       
-      (let length = B.length p in
-      let contents = B.as_seq mem p in
+  (forall p'. disjoint p.b p'.b /\ correct_down_p mem addrs heap p' ==>       
+      (let length = B.length p.b in
+      let contents = B.as_seq mem p.b in
       let addr = addrs p in
       let new_heap = write_vale_mem contents length addr 0 heap in
       correct_down_p mem addrs new_heap p')) = 
   let rec aux (p':b8) : Lemma 
-    (disjoint p p' /\ correct_down_p mem addrs heap p' ==> (let length = B.length p in
-      let contents = B.as_seq mem p in
+    (disjoint p.b p'.b /\ correct_down_p mem addrs heap p' ==> (let length = B.length p.b in
+      let contents = B.as_seq mem p.b in
       let addr = addrs p in
       let new_heap = write_vale_mem contents length addr 0 heap in
       correct_down_p mem addrs new_heap p')) =
-        let length = B.length p in
-        let contents = B.as_seq mem p in
+        let length = B.length p.b in
+        let contents = B.as_seq mem p.b in
         let addr = addrs p in
         let new_heap = write_vale_mem contents length addr 0 heap in
 	frame_write_vale_mem contents length addr 0 heap
   in
   Classical.forall_intro aux
 
-
-
 private let add_buffer_domain (b:b8) (addrs:addr_map) (accu:Set.set int) : GTot (s:Set.set int{
-  forall x. Set.mem x s <==> (Set.mem x accu \/ (x >= addrs b /\ x < addrs b + B.length b))}) =
-  let rec aux (j:nat{j <= B.length b}) (acc:Set.set int{forall x. Set.mem x acc <==>
+  forall x. Set.mem x s <==> (Set.mem x accu \/ (x >= addrs b /\ x < addrs b + B.length b.b))}) =
+  let rec aux (j:nat{j <= B.length b.b}) (acc:Set.set int{forall x. Set.mem x acc <==>
     Set.mem x accu \/ (x >= addrs b /\ x < addrs b + j)}) :
     GTot (s:Set.set int{forall x. Set.mem x s <==>
-    Set.mem x accu \/ (x >= addrs b /\ x < addrs b + B.length b)}) 
-    (decreases %[B.length b - j]) = 
-    if j >= B.length b then acc else begin
+    Set.mem x accu \/ (x >= addrs b /\ x < addrs b + B.length b.b)}) 
+    (decreases %[B.length b.b - j]) = 
+    if j >= B.length b.b then acc else begin
       let s = Set.union acc (Set.singleton (addrs b + j)) in
       aux (j+1) s
     end in
@@ -170,9 +175,9 @@ private let rec addrs_set_aux (ptrs:list b8)
 			      (ps:list b8{forall b. List.memP b ptrs <==> List.memP b ps \/ List.memP b ps2})
 			      (addrs:addr_map)
 			      (accu:Set.set int{forall (x:int). not (Set.mem x accu) <==>
-			        (forall (b:b8{List.memP b ps}). x < addrs b \/ x >= addrs b + B.length b)}) :
+			        (forall (b:b8{List.memP b ps}). x < addrs b \/ x >= addrs b + B.length b.b)}) :
 			 GTot (s:Set.set int{forall (x:int). not (Set.mem x s) <==>
-			        (forall (b:b8{List.memP b ptrs}). x < addrs b \/ x >= addrs b + B.length b)}) =
+			        (forall (b:b8{List.memP b ptrs}). x < addrs b \/ x >= addrs b + B.length b.b)}) =
   match ps2 with
   | [] -> accu
   | a::q -> 
@@ -181,7 +186,7 @@ private let rec addrs_set_aux (ptrs:list b8)
       (requires True)
       (ensures not (Set.mem x s) <==> 
       (forall (b:b8{List.memP b (a::ps)}). 
-	x < addrs b \/ x >= addrs b + B.length b)) = ()
+	x < addrs b \/ x >= addrs b + B.length b.b)) = ()
     in
     Classical.forall_intro aux;
     addrs_set_aux ptrs q (a::ps) addrs s
@@ -202,8 +207,8 @@ let addrs_set_concat ptrs a addrs =
 let addrs_set_mem ptrs a addrs i = ()
 
 let write_buffer_vale (a:b8) (heap:heap) (mem:HS.mem) (addrs:addr_map) =
-  let length = B.length a in
-  let contents = B.as_seq mem a in
+  let length = B.length a.b in
+  let contents = B.as_seq mem a.b in
   let addr = addrs a in
   write_vale_mem contents length addr 0 heap
 
@@ -214,8 +219,8 @@ let domain_write_buffer (a:b8) (heap:heap) (mem:HS.mem) (addrs:addr_map) : Lemma
    let s1 = Map.domain heap in
    let s2 = addrs_set [a] addrs in
    let s3 = Map.domain new_heap in
-   let length = B.length a in
-   let contents = B.as_seq mem a in
+   let length = B.length a.b in
+   let contents = B.as_seq mem a.b in
    let addr = addrs a in   
    domain_write_vale_mem contents length addr 0 heap;
    domain2_write_vale_mem contents length addr 0 heap;
@@ -233,15 +238,14 @@ let rec down_mem_aux (ptrs:list b8{list_disjoint_or_eq ptrs})
     | [] -> addrs_set_lemma accu ptrs addrs; h
     | a::q ->
       let new_heap = write_buffer_vale a h mem addrs in
-      let length = B.length a in
-      let contents = B.as_seq mem a in
+      let length = B.length a.b in
+      let contents = B.as_seq mem a.b in
       let addr = addrs a in      
       load_store_write_vale_mem contents length addr 0 h;
       correct_down_p_cancel mem addrs h a;
       correct_down_p_frame mem addrs h a;
-      assert (forall p. List.memP p accu ==> disjoint_or_eq p a);
+      assert (forall (p:b8). List.memP p accu ==> disjoint_or_eq p.b a.b);
       domain_write_buffer a h mem addrs;
-      addrs_set_concat accu a addrs;
       down_mem_aux ptrs addrs mem q (a::accu) new_heap
 
 let down_mem mem addrs ptrs =
@@ -260,19 +264,19 @@ let rec frame_down_mem_aux (ptrs:list b8{list_disjoint_or_eq ptrs})
   (let heap = down_mem_aux ptrs addrs mem ps accu h in
    forall i. (forall (b:b8{List.memP b ptrs}). 
       let base = addrs b in
-      i < base \/ i >= base + B.length b) ==>
+      i < base \/ i >= base + B.length b.b) ==>
       h.[i] == heap.[i]) =
   match ps with
   | [] -> ()
   | a::q ->
     let new_heap = write_buffer_vale a h mem addrs in
-    let length = B.length a in
-    let contents = B.as_seq mem a in
+    let length = B.length a.b in
+    let contents = B.as_seq mem a.b in
     let addr = addrs a in     
     load_store_write_vale_mem contents length addr 0 h;
     correct_down_p_cancel mem addrs h a;
     correct_down_p_frame mem addrs h a;
-    assert (forall p. List.memP p accu ==> disjoint_or_eq p a);
+    assert (forall p. List.memP p accu ==> disjoint_or_eq p.b a.b);
     domain_write_buffer a h mem addrs;
     addrs_set_concat accu a addrs;
     let new_heap' = down_mem_aux ptrs addrs mem q (a::accu) new_heap in
@@ -294,9 +298,9 @@ let same_unspecified_down mem1 mem2 addrs ptrs =
 
 let get_seq_heap_as_seq (heap1 heap2:heap) (addrs:addr_map) (mem:HS.mem) (b:b8) : Lemma
   (requires correct_down_p mem addrs heap1 b /\
-    (forall x. x >= addrs b /\ x < addrs b + B.length b ==> heap1.[x] == heap2.[x]))
-  (ensures B.as_seq mem b == get_seq_heap heap2 addrs b) =
-  assert (Seq.equal (B.as_seq mem b) (get_seq_heap heap2 addrs b))
+    (forall x. x >= addrs b /\ x < addrs b + B.length b.b ==> heap1.[x] == heap2.[x]))
+  (ensures B.as_seq mem b.b == get_seq_heap heap2 addrs b) =
+  assert (Seq.equal (B.as_seq mem b.b) (get_seq_heap heap2 addrs b))
 
 let rec up_mem_aux (heap:heap)
                (addrs:addr_map)
@@ -311,8 +315,8 @@ let rec up_mem_aux (heap:heap)
     | [] -> m
     | a::q ->
       let s = get_seq_heap heap addrs a in
-      B.g_upd_seq_as_seq a s m;
-      let m' = B.g_upd_seq a s m in
+      B.g_upd_seq_as_seq a.b s m;
+      let m' = B.g_upd_seq a.b s m in
       up_mem_aux heap addrs ptrs q (a::accu) m'
 
 let up_mem heap addrs ptrs mem = up_mem_aux heap addrs ptrs ptrs [] mem
@@ -329,11 +333,11 @@ let rec down_up_identity_aux
   | [] -> ()
   | a::q ->
       let s = get_seq_heap heap addrs a in
-      let m' = B.g_upd_seq a s m in
-      B.lemma_g_upd_with_same_seq a m;
-      assert (Seq.equal s (B.as_seq m a));
+      let m' = B.g_upd_seq a.b s m in
+      B.lemma_g_upd_with_same_seq a.b m;
+      assert (Seq.equal s (B.as_seq m a.b));
       (* The previous assertion and lemma ensure that m == m' *)
-      B.g_upd_seq_as_seq a s m;
+      B.g_upd_seq_as_seq a.b s m;
       down_up_identity_aux heap addrs ptrs q (a::accu) m'
 
 let down_up_identity mem addrs ptrs =
@@ -341,12 +345,13 @@ let down_up_identity mem addrs ptrs =
   down_up_identity_aux heap addrs ptrs ptrs [] mem
 
 let correct_down_p_same_sel (b:b8) (mem:HS.mem) (addrs:addr_map) (heap1 heap2:heap) (x:int) : Lemma
-  (requires (x >= addrs b /\ x < addrs b + B.length b 
+  (requires (x >= addrs b /\ x < addrs b + B.length b.b 
     /\ correct_down_p mem addrs heap1 b /\ correct_down_p mem addrs heap2 b))
   (ensures Map.sel heap1 x == Map.sel heap2 x) = 
     let i = x - addrs b in
     assert (heap1.[x] == heap1.[addrs b + i]);
-    assert (heap2.[x] == heap2.[addrs b + i])
+    assert (heap2.[x] == heap2.[addrs b + i]);
+    assert (heap1.[x] == UInt8.v (Seq.index (B.as_seq mem b.b) i))
 
 let rec up_down_identity_aux
   (ptrs:list b8{list_disjoint_or_eq ptrs})
@@ -386,18 +391,18 @@ let g_upd_tot_correct_down_invariant
   : Lemma
   (requires forall p. (p =!= b /\ List.memP p ptrs) ==> correct_down_p mem addrs heap1 p)
   (ensures (
-    let m' = B.g_upd_seq b (get_seq_heap heap2 addrs b) mem in
+    let m' = B.g_upd_seq b.b (get_seq_heap heap2 addrs b) mem in
     forall p. (p =!= b /\ List.memP p ptrs) ==> correct_down_p m' addrs heap1 p)
   ) = 
-    B.g_upd_seq_as_seq b (get_seq_heap heap2 addrs b) mem
+    B.g_upd_seq_as_seq b.b (get_seq_heap heap2 addrs b) mem
 
 let g_upd_tot_correct_down
   (mem:HS.mem)
   (addrs:addr_map)
   (heap:heap)
-  (b:b8{B.live mem b}) :
-  Lemma (correct_down_p (B.g_upd_seq b (get_seq_heap heap addrs b) mem) addrs heap b) =
-  B.g_upd_seq_as_seq b (get_seq_heap heap addrs b) mem
+  (b:b8{B.live mem b.b}) :
+  Lemma (correct_down_p (B.g_upd_seq b.b (get_seq_heap heap addrs b) mem) addrs heap b) =
+  B.g_upd_seq_as_seq b.b (get_seq_heap heap addrs b) mem
 
 #reset-options "--z3rlimit 50 --max_fuel 1 --max_ifuel 1 --initial_fuel 1 --initial_ifuel 1"
 let rec update_buffer_up_mem_aux
@@ -409,35 +414,42 @@ let rec update_buffer_up_mem_aux
   (heap2:heap{Set.equal (Map.domain heap1) (Map.domain heap2)})
   (ps:list b8)
   (accu:list b8{forall p. List.memP p ptrs <==> List.memP p ps \/ List.memP p accu}) : Lemma
-  (requires (forall x. x < addrs b \/ x >= addrs b + B.length b ==> heap1.[x] == heap2.[x]) /\
-    (List.memP b accu ==> B.as_seq mem b == get_seq_heap heap2 addrs b) /\  
+  (requires (forall x. x < addrs b \/ x >= addrs b + B.length b.b ==> heap1.[x] == heap2.[x]) /\
+    (List.memP b accu ==> B.as_seq mem b.b == get_seq_heap heap2 addrs b) /\  
     (forall p. List.memP p accu ==> correct_down_p mem addrs heap2 p) /\
     (forall p. (p =!= b /\ List.memP p ptrs) ==> correct_down_p mem addrs heap1 p)    )
   (ensures 
   (List.memP b accu ==> up_mem_aux heap2 addrs ptrs ps accu mem == mem) /\
   (~(List.memP b accu) ==> up_mem_aux heap2 addrs ptrs ps accu mem ==
-    B.g_upd_seq b (get_seq_heap heap2 addrs b) mem))
+    B.g_upd_seq b.b (get_seq_heap heap2 addrs b) mem))
   (decreases ps)
   
   = match ps with
    | [] -> ()
    | a::q ->
-     let s = get_seq_heap heap2 addrs a in       
-     B.g_upd_seq_as_seq a s mem;         
-     let m' = B.g_upd_seq a s mem in
+     let s = get_seq_heap heap2 addrs a in
+     B.g_upd_seq_as_seq a.b s mem;         
+     let m' = B.g_upd_seq a.b s mem in
+     let m_f = up_mem_aux heap2 addrs ptrs q (a::accu) m' in
+     // Why is this not verifying, even with an assume?
+     assume (up_mem_aux heap2 addrs ptrs (a::q) accu mem == m_f);
+     admit();
      if StrongExcludedMiddle.strong_excluded_middle (a == b) then (
        if StrongExcludedMiddle.strong_excluded_middle (List.memP b accu) then (
-         B.lemma_g_upd_with_same_seq a mem;       
+         admit();
+         B.lemma_g_upd_with_same_seq a.b mem;       
          update_buffer_up_mem_aux ptrs addrs m' b heap1 heap2 q (a::accu)
        ) else (
+         admit();
          g_upd_tot_correct_down_invariant ptrs addrs heap1 heap2 b mem;
          g_upd_tot_correct_down mem addrs heap2 b;
-         update_buffer_up_mem_aux ptrs addrs m' b heap1 heap2 q (a::accu)
+         update_buffer_up_mem_aux ptrs addrs m' b heap1 heap2 q (a::accu)         
        )
      ) else (
-       assert (B.disjoint a b);
+     admit();
+       assert (B.disjoint a.b b.b);
        get_seq_heap_as_seq heap1 heap2 addrs mem a;
-       B.lemma_g_upd_with_same_seq a mem;       
+       B.lemma_g_upd_with_same_seq a.b mem;       
        update_buffer_up_mem_aux ptrs addrs m' b heap1 heap2 q (a::accu)
      )
 
