vale/code/arch/x64/X64.Memory.fst
@@ -11,7 +11,7 @@ module S = X64.Bytes_Semantics_s
 
 #reset-options "--initial_fuel 2 --max_fuel 2 --initial_ifuel 1 --max_ifuel 1"
 
-let b8 = B.buffer UInt8.t
+let b8 = I.b8
 
 let heap = H.heap
 noeq type mem' = {
